concurrency/machine_semantics.v
@@ -40,11 +40,11 @@ Definition option_proj {A: Type} (default: A) (x: option A) :=
  match x with Some y => y | None => default end.
 
 Record ConcurSemantics {G TID SCH TR C M: Type} : Type :=
-  { initial_machine : G -> M -> val -> list val -> option (C * option M) 
+  { initial_machine : G -> M -> C -> val -> list val -> Prop
     ; conc_halted : SCH -> C -> option val
     ; thread_step : G -> SCH -> C -> M -> C -> M -> Prop
     ; machine_step : G -> SCH -> TR -> C -> M -> SCH -> TR -> C -> M -> Prop
-    ; runing_thread : C -> TID -> Prop
+    ; running_thread : C -> TID -> Prop
     ; thread_step_not_halted:
       forall ge  U m q  m' q', thread_step ge U q m q' m' -> conc_halted U q = None
     ; machine_step_not_halted:
